Size_t and ptrdiff_t types are called t, similarlly to uints

ulib/FStar.SizeT.fst
@@ -6,7 +6,7 @@ module Cast = FStar.Int.Cast
 (* This is only intended as a model, but will be extracted natively by Krml
    with the correct C semantics *)
 
-let size_t = U64.t
+let t = U64.t
 
 let fits x =
   FStar.UInt.fits x U64.n == true
@@ -14,16 +14,16 @@ let fits x =
 let v x =
   U64.v x
 
-let size_v_inj (x1 x2: size_t) = ()
+let size_v_inj (x1 x2: t) = ()
 
-let mk (x: U16.t) : Pure size_t
+let mk (x: U16.t) : Pure t
   (requires True)
   (ensures (fun y -> v y == U16.v x))
 = Cast.uint16_to_uint64 x
 
 let mk_checked x = x
 
-let int_to_size_t x =
+let int_to_t x =
   U64.uint_to_t x
 
 let fits_le x y = ()
