ulib/FStar.PtrdiffT.fst
@@ -2,14 +2,14 @@ module FStar.PtrdiffT
 
 module Cast = FStar.Int.Cast
 
-let ptrdiff_t = I64.t
+let t = I64.t
 
 let fits x = FStar.Int.fits x I64.n == true
 
 let v x =
   I64.v x
 
-let ptrdiff_v_inj (x1 x2: ptrdiff_t) = ()
+let ptrdiff_v_inj (x1 x2: t) = ()
 
 let mk x = Cast.int16_to_int64 x
 let mk_checked x = x
