ulib/FStar.SizeT.fsti
@@ -5,33 +5,33 @@ open FStar.Mul
 module U16 = FStar.UInt16
 module U64 = FStar.UInt64
 
-val size_t : eqtype
+val t : eqtype
 
 val fits (x: nat) : Tot prop
 
-val v (x: size_t) : Ghost nat
+val v (x: t) : Ghost nat
   (requires True)
   (ensures (fun y -> fits y))
 
-val size_v_inj (x1 x2: size_t) : Lemma
+val size_v_inj (x1 x2: t) : Lemma
   (v x1 == v x2 ==> x1 == x2)
   [SMTPat (v x1); SMTPat (v x2)]
 
-/// According to the C standard, "the bit width of size_t is not less than 16 since c99"
-/// (https://en.cppreference.com/w/c/types/size_t)
-/// We therefore offer two functions to create a size_t value.
-/// Any value that fits in a uint_16 can be cast directly to size_t
+/// According to the C standard, "the bit width of t is not less than 16 since c99"
+/// (https://en.cppreference.com/w/c/types/t)
+/// We therefore offer two functions to create a t value.
+/// Any value that fits in a uint_16 can be cast directly to t
 /// Any value that might not fit in a uint_16 needs to be checked,
 /// we will add a static_assert during extraction
-val mk (x: U16.t) : Pure size_t
+val mk (x: U16.t) : Pure t
   (requires True)
   (ensures (fun y -> v y == U16.v x))
 
-val mk_checked (x: U64.t) : Pure size_t
+val mk_checked (x: U64.t) : Pure t
   (requires True)
   (ensures (fun y -> v y == U64.v x))
 
-val int_to_size_t (x: nat) : Ghost size_t
+val int_to_t (x: nat) : Ghost t
   (requires (fits x))
   (ensures (fun y -> v y == x))
 
@@ -40,22 +40,22 @@ val fits_le (x y: nat) : Lemma
   (ensures (fits x))
   [SMTPat (fits x); SMTPat (fits y)]
 
-val add (x y: size_t) : Pure size_t
+val add (x y: t) : Pure t
   (requires (fits (v x + v y)))
   (ensures (fun z -> v z == v x + v y))
 
-val sub (x y: size_t) : Pure size_t
+val sub (x y: t) : Pure t
   (requires (v x >= v y))
   (ensures (fun z -> v z == v x - v y))
 
-val mul (x y: size_t) : Pure size_t
+val mul (x y: t) : Pure t
   (requires (fits (v x * v y)))
   (ensures (fun z -> v z == v x * v y))
 
-val le (x y: size_t) : Pure bool
+val le (x y: t) : Pure bool
   (requires True)
   (ensures (fun z -> z == (v x <= v y)))
 
-let zero : (zero_size: size_t { v zero_size == 0 }) = mk 0us
+let zero : (zero_size: t { v zero_size == 0 }) = mk 0us
 
-let one : (zero_size: size_t { v zero_size == 1 }) = mk 1us
+let one : (zero_size: t { v zero_size == 1 }) = mk 1us
